proof/iu_system/uni/decl/def_extra.v
@@ -22,88 +22,88 @@ end.
 
 (* defns Jd_wf_typ_s *)
 Inductive d_wf_typ_s : denv -> typ -> Prop :=    (* defn d_wf_typ_s *)
- | dwftyps_unit : forall (E:denv),
-     d_wf_typ_s E typ_unit
- | dwftyps_bot : forall (E:denv),
-     d_wf_typ_s E typ_bot
- | dwftyps_top : forall (E:denv),
-     d_wf_typ_s E typ_top
- | dwftyps_var : forall (E:denv) (X:typvar),
-      binds ( X )  ( dbind_tvar_empty ) ( E )  ->
-     d_wf_typ_s E (typ_var_f X)
- | dwftyps_stvar : forall (E:denv) (X:typvar),
-      binds ( X ) ( dbind_stvar_empty ) ( E )  ->
-     d_wf_typ_s E (typ_var_f X)
- | dwftyps_arrow : forall (E:denv) (T1 T2:typ),
-     d_wf_typ_s E T1 ->
-     d_wf_typ_s E T2 ->
-     d_wf_typ_s E (typ_arrow T1 T2)
- | dwftyps_all : forall (L:vars) (E:denv) (T1:typ),
+ | dwftyps_unit : forall (Ψ:denv),
+     d_wf_typ_s Ψ typ_unit
+ | dwftyps_bot : forall (Ψ:denv),
+     d_wf_typ_s Ψ typ_bot
+ | dwftyps_top : forall (Ψ:denv),
+     d_wf_typ_s Ψ typ_top
+ | dwftyps_var : forall (Ψ:denv) (X:typvar),
+      binds ( X )  ( dbind_tvar_empty ) ( Ψ )  ->
+     d_wf_typ_s Ψ (typ_var_f X)
+ | dwftyps_stvar : forall (Ψ:denv) (X:typvar),
+      binds ( X ) ( dbind_stvar_empty ) ( Ψ )  ->
+     d_wf_typ_s Ψ (typ_var_f X)
+ | dwftyps_arrow : forall (Ψ:denv) (T1 T2:typ),
+     d_wf_typ_s Ψ T1 ->
+     d_wf_typ_s Ψ T2 ->
+     d_wf_typ_s Ψ (typ_arrow T1 T2)
+ | dwftyps_all : forall (L:vars) (Ψ:denv) (T1:typ),
      ( forall X , X \notin L -> ds_in X  (open_typ_wrt_typ  T1   (typ_var_f X) ) ) ->
-     ( forall X , X \notin L -> d_wf_typ_s  ( X ~ dbind_stvar_empty  ++  E )   (open_typ_wrt_typ  T1   (typ_var_f X) ) ) ->
-     d_wf_typ_s E (typ_all T1)
- | dwftyps_union : forall (E:denv) (T1 T2:typ),
-     d_wf_typ_s E T1 ->
-     d_wf_typ_s E T2 ->
-     d_wf_typ_s E (typ_union T1 T2)
- | dwftyps_intersection : forall (E:denv) (T1 T2:typ),
-     d_wf_typ_s E T1 ->
-     d_wf_typ_s E T2 ->
-     d_wf_typ_s E (typ_intersection T1 T2).
+     ( forall X , X \notin L -> d_wf_typ_s  ( X ~ dbind_stvar_empty  ++  Ψ )   (open_typ_wrt_typ  T1   (typ_var_f X) ) ) ->
+     d_wf_typ_s Ψ (typ_all T1)
+ | dwftyps_union : forall (Ψ:denv) (T1 T2:typ),
+     d_wf_typ_s Ψ T1 ->
+     d_wf_typ_s Ψ T2 ->
+     d_wf_typ_s Ψ (typ_union T1 T2)
+ | dwftyps_intersection : forall (Ψ:denv) (T1 T2:typ),
+     d_wf_typ_s Ψ T1 ->
+     d_wf_typ_s Ψ T2 ->
+     d_wf_typ_s Ψ (typ_intersection T1 T2).
 
 
 Inductive d_inftapp : denv -> typ -> typ -> typ -> Prop := 
-| d_inftapp__bot : forall (E:denv) (T1:typ),
-    d_wf_env E -> 
-    d_wf_typ E T1 ->
-    d_inftapp E typ_bot T1 typ_bot
-| d_inftapp__all : forall (E:denv) (T1 T2:typ),
-    d_wf_env E -> 
-    d_wf_typ E (typ_all T1) ->
-    d_wf_typ E T2 ->
-    d_inftapp E (typ_all T1) T2 (open_typ_wrt_typ  T1   T2 )
-| d_inftapp__intersection1 : forall (E:denv) (A1 A2 B C1:typ),
-    d_wf_typ E A2 ->
-    d_inftapp E A1 B C1 ->
-    d_inftapp E (typ_intersection A1 A2) B C1
-| d_inftapp__intersection2 : forall (E:denv) (A1 A2 B C2:typ),
-    d_wf_typ E A1 ->
-    d_inftapp E A2 B C2 ->
-    d_inftapp E (typ_intersection A1 A2) B C2
-| d_typing__union : forall (E:denv) (A1 A2 B C1 C2:typ),
-    d_inftapp E A1 B C1 ->
-    d_inftapp E A2 B C2 ->
-    d_inftapp E (typ_union A1 A2) B (typ_union C1 C2)
+| d_inftapp__bot : forall (Ψ:denv) (T1:typ),
+    d_wf_env Ψ -> 
+    d_wf_typ Ψ T1 ->
+    d_inftapp Ψ typ_bot T1 typ_bot
+| d_inftapp__all : forall (Ψ:denv) (T1 T2:typ),
+    d_wf_env Ψ -> 
+    d_wf_typ Ψ (typ_all T1) ->
+    d_wf_typ Ψ T2 ->
+    d_inftapp Ψ (typ_all T1) T2 (open_typ_wrt_typ  T1   T2 )
+| d_inftapp__intersection1 : forall (Ψ:denv) (A1 A2 B C1:typ),
+    d_wf_typ Ψ A2 ->
+    d_inftapp Ψ A1 B C1 ->
+    d_inftapp Ψ (typ_intersection A1 A2) B C1
+| d_inftapp__intersection2 : forall (Ψ:denv) (A1 A2 B C2:typ),
+    d_wf_typ Ψ A1 ->
+    d_inftapp Ψ A2 B C2 ->
+    d_inftapp Ψ (typ_intersection A1 A2) B C2
+| d_typing__union : forall (Ψ:denv) (A1 A2 B C1 C2:typ),
+    d_inftapp Ψ A1 B C1 ->
+    d_inftapp Ψ A2 B C2 ->
+    d_inftapp Ψ (typ_union A1 A2) B (typ_union C1 C2)
 .
 
 
 Inductive d_infabs : denv -> typ -> typ -> typ -> Prop := 
-| d_infabs__bot : forall (E:denv),
-    d_wf_env E ->
-    d_infabs E typ_bot typ_top typ_bot
-| d_infabs__arr : forall (E:denv) (T1 T2:typ),
-    d_wf_env E ->
-    d_wf_typ E T1 ->
-    d_wf_typ E T2 ->
-    d_infabs E (typ_arrow T1 T2) T1 T2
-| d_infabs__all : forall (E:denv) (T1 T2 T3 T4:typ),
-    d_mono_typ E T2 -> 
-    d_wf_typ E T2 ->
-    d_wf_typ E (typ_all T1) ->
-    d_infabs E  (open_typ_wrt_typ  T1   T2 ) T3 T4 ->
-    d_infabs E (typ_all T1) T3 T4
-| d_infabs__intersection1 : forall (E:denv) (T1 T2 T3 T4:typ),
-    d_wf_typ E T2 ->
-    d_infabs E T1 T3 T4->
-    d_infabs E (typ_intersection T1 T2) T3 T4
-| d_infabs__intersection2 : forall (E:denv) (T1 T2 T3 T4:typ),
-    d_wf_typ E T1 ->
-    d_infabs E T2 T3 T4->
-    d_infabs E (typ_intersection T1 T2) T3 T4
-| d_infabs__union : forall (E:denv) (T1 T2 T3 T4 T5 T6:typ),
-    d_infabs E T1 T3 T4->
-    d_infabs E T2 T5 T6->
-    d_infabs E (typ_union T1 T2) (typ_intersection T3 T5) (typ_union T4 T6)
+| d_infabs__bot : forall (Ψ:denv),
+    d_wf_env Ψ ->
+    d_infabs Ψ typ_bot typ_top typ_bot
+| d_infabs__arr : forall (Ψ:denv) (T1 T2:typ),
+    d_wf_env Ψ ->
+    d_wf_typ Ψ T1 ->
+    d_wf_typ Ψ T2 ->
+    d_infabs Ψ (typ_arrow T1 T2) T1 T2
+| d_infabs__all : forall (Ψ:denv) (T1 T2 T3 T4:typ),
+    d_mono_typ Ψ T2 -> 
+    d_wf_typ Ψ T2 ->
+    d_wf_typ Ψ (typ_all T1) ->
+    d_infabs Ψ  (open_typ_wrt_typ  T1   T2 ) T3 T4 ->
+    d_infabs Ψ (typ_all T1) T3 T4
+| d_infabs__intersection1 : forall (Ψ:denv) (T1 T2 T3 T4:typ),
+    d_wf_typ Ψ T2 ->
+    d_infabs Ψ T1 T3 T4->
+    d_infabs Ψ (typ_intersection T1 T2) T3 T4
+| d_infabs__intersection2 : forall (Ψ:denv) (T1 T2 T3 T4:typ),
+    d_wf_typ Ψ T1 ->
+    d_infabs Ψ T2 T3 T4->
+    d_infabs Ψ (typ_intersection T1 T2) T3 T4
+| d_infabs__union : forall (Ψ:denv) (T1 T2 T3 T4 T5 T6:typ),
+    d_infabs Ψ T1 T3 T4->
+    d_infabs Ψ T2 T5 T6->
+    d_infabs Ψ (typ_union T1 T2) (typ_intersection T3 T5) (typ_union T4 T6)
 .
 
 Inductive typing_mode :=
@@ -111,56 +111,56 @@ Inductive typing_mode :=
 | typingmode__chk.
 
 Inductive d_typing : denv -> exp -> typing_mode -> typ -> Prop :=
-| d_typing__infvar : forall (E:denv) (x:expvar) (T1:typ),
-    d_wf_env E ->
-    binds ( x )  ( (dbind_typ T1) ) ( E )  ->
-    d_typing E (exp_var_f x) typingmode__inf T1
-| d_typing__infanno : forall (E:denv) (e:exp) (T1:typ),
-    d_wf_typ E T1 ->
-    d_typing E e typingmode__chk T1 ->
-    d_typing E  ( (exp_anno e T1) )  typingmode__inf T1
-| d_typinginf_unit : forall (E:denv),
-    d_wf_env E ->
-    d_typing E exp_unit typingmode__inf typ_unit
-| d_typing__infapp : forall (E:denv) (e1 e2:exp) (T1 T2 T3:typ),
-    d_typing E e1 typingmode__inf T1 ->
-    d_infabs E T1 T2 T3 ->
-    d_typing E e2 typingmode__chk T2 ->
-    d_typing E  ( (exp_app e1 e2) ) typingmode__inf T3
-| d_typing__inftabs : forall (L:vars) (E:denv) (e:exp) (T1:typ),
-d_wf_typ E (typ_all T1) ->
-    ( forall X , X \notin  L  -> d_typing  ( X ~ dbind_tvar_empty  ++  E ) (exp_anno  ( open_exp_wrt_typ e (typ_var_f X) )  ( open_typ_wrt_typ T1 (typ_var_f X) ) ) typingmode__chk ( open_typ_wrt_typ T1 (typ_var_f X) )  )  ->
-    d_typing E (exp_tabs (body_anno e T1)) typingmode__inf (typ_all T1)
-| d_typing__inftapp : forall (E:denv) (e1:exp) (T1 T2 T3:typ),
-    d_wf_typ E T2 ->
-    d_typing E e1 typingmode__inf T1 ->
-    d_inftapp E T1 T2 T3 ->
-    d_typing E (exp_tapp e1 T2) typingmode__inf T3
-| d_typing__chkabstop : forall (L:vars) (E:denv) (e:exp),
-    ( forall x , x \notin  L  -> d_typing  ( x ~ (dbind_typ typ_bot)  ++  E )   ( open_exp_wrt_exp e (exp_var_f x) ) typingmode__chk typ_top )  ->
-    d_typing E (exp_abs e) typingmode__chk typ_top
-| d_typing__chkabs : forall (L:vars) (E:denv) (e:exp) (T1 T2:typ),
-    d_wf_typ E T1 ->
-    ( forall x , x \notin  L  -> d_typing  ( x ~ (dbind_typ T1)  ++  E )  ( open_exp_wrt_exp e (exp_var_f x) ) typingmode__chk T2 )  ->
-    d_typing E (exp_abs e) typingmode__chk (typ_arrow T1 T2)
-(* | d_typing__chkall : forall (L:vars) (E:denv) (e:exp) (T1:typ),
-    d_wf_typ E (typ_all T1) ->
-    ( forall X , X \notin  L  -> d_typing  ( X ~ dbind_tvar_empty  ++  E )  e  typingmode__chk ( open_typ_wrt_typ T1 (typ_var_f X) )  )  ->
-    d_typing E e typingmode__chk (typ_all T1) *)
-| d_typing__chksub : forall (E:denv) (e:exp) (T1 S1:typ),
-    d_typing E e typingmode__inf S1 ->
-    d_sub E S1 T1 ->
-    d_typing E e typingmode__chk T1
-| d_typing__chkintersection : forall (E:denv) (e:exp) (S1 T1:typ),
-    d_typing E e typingmode__chk S1 ->
-    d_typing E e typingmode__chk T1 ->
-    d_typing E e typingmode__chk (typ_intersection S1 T1)
-| d_typing__chkunion1 : forall (E:denv) (e:exp) (S1 T1:typ),
-    d_typing E e typingmode__chk S1 ->
-    d_wf_typ E T1 ->
-    d_typing E e typingmode__chk (typ_union S1 T1)
-| d_typing__chkunion2 : forall (E:denv) (e:exp) (S1 T1:typ),
-    d_typing E e typingmode__chk T1 ->
-    d_wf_typ E S1 ->
-    d_typing E e typingmode__chk (typ_union S1 T1)
+| d_typing__infvar : forall (Ψ:denv) (x:expvar) (T1:typ),
+    d_wf_env Ψ ->
+    binds ( x )  ( (dbind_typ T1) ) ( Ψ )  ->
+    d_typing Ψ (exp_var_f x) typingmode__inf T1
+| d_typing__infanno : forall (Ψ:denv) (e:exp) (T1:typ),
+    d_wf_typ Ψ T1 ->
+    d_typing Ψ e typingmode__chk T1 ->
+    d_typing Ψ  ( (exp_anno e T1) )  typingmode__inf T1
+| d_typinginf_unit : forall (Ψ:denv),
+    d_wf_env Ψ ->
+    d_typing Ψ exp_unit typingmode__inf typ_unit
+| d_typing__infapp : forall (Ψ:denv) (e1 e2:exp) (T1 T2 T3:typ),
+    d_typing Ψ e1 typingmode__inf T1 ->
+    d_infabs Ψ T1 T2 T3 ->
+    d_typing Ψ e2 typingmode__chk T2 ->
+    d_typing Ψ  ( (exp_app e1 e2) ) typingmode__inf T3
+| d_typing__inftabs : forall (L:vars) (Ψ:denv) (e:exp) (T1:typ),
+d_wf_typ Ψ (typ_all T1) ->
+    ( forall X , X \notin  L  -> d_typing  ( X ~ dbind_tvar_empty  ++  Ψ ) (exp_anno  ( open_exp_wrt_typ e (typ_var_f X) )  ( open_typ_wrt_typ T1 (typ_var_f X) ) ) typingmode__chk ( open_typ_wrt_typ T1 (typ_var_f X) )  )  ->
+    d_typing Ψ (exp_tabs (body_anno e T1)) typingmode__inf (typ_all T1)
+| d_typing__inftapp : forall (Ψ:denv) (e1:exp) (T1 T2 T3:typ),
+    d_wf_typ Ψ T2 ->
+    d_typing Ψ e1 typingmode__inf T1 ->
+    d_inftapp Ψ T1 T2 T3 ->
+    d_typing Ψ (exp_tapp e1 T2) typingmode__inf T3
+| d_typing__chkabstop : forall (L:vars) (Ψ:denv) (e:exp),
+    ( forall x , x \notin  L  -> d_typing  ( x ~ (dbind_typ typ_bot)  ++  Ψ )   ( open_exp_wrt_exp e (exp_var_f x) ) typingmode__chk typ_top )  ->
+    d_typing Ψ (exp_abs e) typingmode__chk typ_top
+| d_typing__chkabs : forall (L:vars) (Ψ:denv) (e:exp) (T1 T2:typ),
+    d_wf_typ Ψ T1 ->
+    ( forall x , x \notin  L  -> d_typing  ( x ~ (dbind_typ T1)  ++  Ψ )  ( open_exp_wrt_exp e (exp_var_f x) ) typingmode__chk T2 )  ->
+    d_typing Ψ (exp_abs e) typingmode__chk (typ_arrow T1 T2)
+(* | d_typing__chkall : forall (L:vars) (Ψ:denv) (e:exp) (T1:typ),
+    d_wf_typ Ψ (typ_all T1) ->
+    ( forall X , X \notin  L  -> d_typing  ( X ~ dbind_tvar_empty  ++  Ψ )  e  typingmode__chk ( open_typ_wrt_typ T1 (typ_var_f X) )  )  ->
+    d_typing Ψ e typingmode__chk (typ_all T1) *)
+| d_typing__chksub : forall (Ψ:denv) (e:exp) (T1 S1:typ),
+    d_typing Ψ e typingmode__inf S1 ->
+    d_sub Ψ S1 T1 ->
+    d_typing Ψ e typingmode__chk T1
+| d_typing__chkintersection : forall (Ψ:denv) (e:exp) (S1 T1:typ),
+    d_typing Ψ e typingmode__chk S1 ->
+    d_typing Ψ e typingmode__chk T1 ->
+    d_typing Ψ e typingmode__chk (typ_intersection S1 T1)
+| d_typing__chkunion1 : forall (Ψ:denv) (e:exp) (S1 T1:typ),
+    d_typing Ψ e typingmode__chk S1 ->
+    d_wf_typ Ψ T1 ->
+    d_typing Ψ e typingmode__chk (typ_union S1 T1)
+| d_typing__chkunion2 : forall (Ψ:denv) (e:exp) (S1 T1:typ),
+    d_typing Ψ e typingmode__chk T1 ->
+    d_wf_typ Ψ S1 ->
+    d_typing Ψ e typingmode__chk (typ_union S1 T1)
 .
